change ListMemory from word to mword addresses

src/ListMemory.v
@@ -46,66 +46,65 @@ Proof.
 Qed.
 
 
-(* bitwidth w is ignored on RHS, but we still want to carry it in the type *)
-Definition mem(w: nat) := ListMemoryZAddr.mem.
+Definition mem := ListMemoryZAddr.mem.
 
 Section Memory.
 
-  Context {w: nat}. (* bit width of memory addresses *)
+  Context {mword: Set}.
+  Context {MW: MachineWidth mword}.
 
-  Definition mem_size(m: mem w): Z :=
-    align 8 (Z.min (2 ^ Z.of_nat w) (ListMemoryZAddr.mem_size m)).
+  Definition mem_size(m: mem): Z :=
+    align 8 (Z.min (2 ^ XLEN) (ListMemoryZAddr.mem_size m)).
 
-  Definition read_byte(m: mem w)(a: word w): word 8 :=
-    ListMemoryZAddr.read_byte m (uwordToZ a).
+  Definition read_byte(m: mem)(a: mword): word 8 :=
+    ListMemoryZAddr.read_byte m (regToZ_unsigned a).
 
-  Definition read_half(m: mem w)(a: word w): word 16 :=
-    ListMemoryZAddr.read_half m (uwordToZ a).
+  Definition read_half(m: mem)(a: mword): word 16 :=
+    ListMemoryZAddr.read_half m (regToZ_unsigned a).
 
-  Definition read_word(m: mem w)(a: word w): word 32 :=
-    ListMemoryZAddr.read_word m (uwordToZ a).
+  Definition read_word(m: mem)(a: mword): word 32 :=
+    ListMemoryZAddr.read_word m (regToZ_unsigned a).
 
-  Definition read_double(m: mem w)(a: word w): word 64 :=
-    ListMemoryZAddr.read_double m (uwordToZ a).
+  Definition read_double(m: mem)(a: mword): word 64 :=
+    ListMemoryZAddr.read_double m (regToZ_unsigned a).
 
-  Definition write_byte(m: mem w)(a: word w)(v: word 8): mem w :=
-    ListMemoryZAddr.write_byte m (uwordToZ a) v.
+  Definition write_byte(m: mem)(a: mword)(v: word 8): mem :=
+    ListMemoryZAddr.write_byte m (regToZ_unsigned a) v.
 
-  Definition write_half(m: mem w)(a: word w)(v: word 16): mem w :=
-    ListMemoryZAddr.write_half m (uwordToZ a) v.
+  Definition write_half(m: mem)(a: mword)(v: word 16): mem :=
+    ListMemoryZAddr.write_half m (regToZ_unsigned a) v.
 
-  Definition write_word(m: mem w)(a: word w)(v: word 32): mem w :=
-    ListMemoryZAddr.write_word m (uwordToZ a) v.
+  Definition write_word(m: mem)(a: mword)(v: word 32): mem :=
+    ListMemoryZAddr.write_word m (regToZ_unsigned a) v.
 
-  Definition write_double(m: mem w)(a: word w)(v: word 64): mem w :=
-    ListMemoryZAddr.write_double m (uwordToZ a) v.
+  Definition write_double(m: mem)(a: mword)(v: word 64): mem :=
+    ListMemoryZAddr.write_double m (regToZ_unsigned a) v.
 
-  Definition const_mem(default: word 8)(size: Z): mem w :=
+  Definition const_mem(default: word 8)(size: Z): mem :=
     ListMemoryZAddr.const_mem default size.
 
-  Definition zero_mem: Z -> mem w := const_mem $0.
+  Definition zero_mem: Z -> mem := const_mem $0.
 
   (* Since mem_size is a bit fancy, we better prove that it's possible to create memory of any
      desired size (as long as it's a multiple of 8 and not bigger than the biggest address) *)
   Lemma const_mem_mem_size: forall size default,
       size mod 8 = 0 ->
-      0 <= size <= 2 ^ Z.of_nat w ->
+      0 <= size <= 2 ^ XLEN ->
       mem_size (const_mem default size) = size.
   Proof.
     intros. unfold mem_size, const_mem. rewrite ListMemoryZAddr.const_mem_mem_size by omega.
-    replace (Z.min (2 ^ Z.of_nat w) size) with size by momega.
+    replace (Z.min (2 ^ XLEN) size) with size by momega.
     apply align8_eq. assumption.
   Qed.
 
 End Memory.
 
-Ltac pose_align8_lt :=
+Ltac pose_bounds :=
   repeat match goal with
          | _: context [align 8 ?x] |- _=> unique pose proof (align8_lt x)
          | |- context [align 8 ?x]     => unique pose proof (align8_lt x)
+         | w: _ |- _ => unique pose proof (regToZ_unsigned_bounds w)
          end.
-
-Definition TODO{T: Type}: T. Admitted.
 
 Local Ltac wrap L :=
   intros;
@@ -115,12 +114,11 @@ Local Ltac wrap L :=
   unfold mem_size, ListMemoryZAddr.mem_size in *;
   first [do 2 f_equal; apply L | apply L];
   unfold ListMemoryZAddr.mem_size;
-  pose_align8_lt;
-  try apply wordToNat_neq1;
-  (congruence || momega || apply TODO).
+  pose_bounds;
+  try apply ne_regToZ_unsigned;
+  (congruence || momega || idtac).
 
-Instance mem_is_Memory(w: nat){MW: MachineWidth (word w)}(E: Z.of_nat w = XLEN)
-: Memory (mem w) (word w) := 
+Instance mem_is_Memory(mword: Set){MW: MachineWidth mword}: Memory mem mword := 
 {|
   memSize     := mem_size;
   loadByte    := read_byte;
@@ -132,9 +130,7 @@ Instance mem_is_Memory(w: nat){MW: MachineWidth (word w)}(E: Z.of_nat w = XLEN)
   storeWord   := write_word;
   storeDouble := write_double;
 |}.
-- intros. unfold mem_size. pose_align8_lt.
-  rewrite E in *.
-  momega.
+- intros. unfold mem_size. pose_bounds. momega.
 - intros. unfold mem_size, align. rewrite Z.mul_comm. apply Z.mod_mul. congruence.
 - wrap ListMemoryZAddr.write_read_byte_eq.
 - wrap ListMemoryZAddr.write_read_byte_ne.
@@ -148,19 +144,10 @@ Instance mem_is_Memory(w: nat){MW: MachineWidth (word w)}(E: Z.of_nat w = XLEN)
 - wrap ListMemoryZAddr.write_read_double_eq.
 - wrap ListMemoryZAddr.write_read_double_ne.
 - wrap ListMemoryZAddr.write_double_preserves_mem_size.
-- apply TODO.
-- apply TODO.
-- apply TODO.
-(*
-- unfold read_byte.
-  intros. unfold valid_addr, mem_size in *. pose_align8_lt. rewrite uwordToZ_wplus'' by momega. reflexivity.
-- unfold read_half.
-  intros. unfold valid_addr, mem_size in *. pose_align8_lt. rewrite uwordToZ_wplus'' by momega. reflexivity.
-- unfold read_word.
-  intros. unfold valid_addr, mem_size in *. pose_align8_lt. rewrite uwordToZ_wplus'' by momega. reflexivity.
-*)
+- intros. unfold valid_addr, mem_size, read_byte in *. pose_bounds.
+  rewrite regToZ_unsigned_add_r by momega. reflexivity.
+- intros. unfold valid_addr, mem_size, read_half in *. pose_bounds.
+  rewrite regToZ_unsigned_add_r by momega. reflexivity.
+- intros. unfold valid_addr, mem_size, read_word in *. pose_bounds.
+  rewrite regToZ_unsigned_add_r by momega. reflexivity.
 Defined.
-
-Require Import riscv.MachineWidth32.
-
-Instance mem32_is_Memory: Memory (mem 32) (word 32) := mem_is_Memory _ eq_refl.
